rocq/theories/DetTheories.v
@@ -1,0 +1,77 @@
+Require Import Basic Lang Determinism Trace.
+Require Import BaseTheory.
+Require Import TraceTheories.
+From Coq Require Import Equality Relations RelationClasses List Compare Sets.Ensembles Streams Setoid Classes.Morphisms.
+Import ListNotations.
+
+Module Type DetTheories (B : Basic) (LD : LangDefs) (TD : TraceDefs B LD) (DD : DeterminismDef LD) (TT : TraceTheories B LD TD).
+  Import B LD TD DD TT.
+  Import LangNotations.
+
+  Theorem Eq_EvtSt_refl : forall s: EvtStream, Eq_EvtSt s s.
+    cofix CH.
+    intros.
+    destruct s; constructor; try reflexivity.
+    apply CH.
+  Qed.
+
+  Theorem Eq_EvtSt_sym : forall s1 s2: EvtStream, Eq_EvtSt s1 s2 -> Eq_EvtSt s2 s1.
+    cofix CH.
+    intros.
+    destruct H; [apply Eq_EvtSt_refl | constructor].
+    - rewrite H; reflexivity.
+    - apply CH.
+      assumption.
+  Qed.
+
+  Theorem Eq_EvtSt_trans : forall s1 s2 s3 : EvtStream, Eq_EvtSt s1 s2 -> Eq_EvtSt s2 s3 -> Eq_EvtSt s1 s3.
+    cofix CH.
+    intros ? ? ? H12 H23.
+    destruct H12 eqn:Heqn.
+    - destruct s3.
+      + inversion H23.
+      + apply Eq_EvtSt_refl.
+    - destruct s3; inversion H23.
+      + subst; constructor; [reflexivity | ].
+        apply (CH t1 t2 s3); assumption.
+  Qed.  
+
+  Instance Eq_EvtSt_equiv: Equivalence (Eq_EvtSt).
+    Proof.
+      constructor.
+      - exact Eq_EvtSt_refl.
+      - exact Eq_EvtSt_sym.
+      - exact Eq_EvtSt_trans.
+    Qed.
+
+    Global Instance EvtCons_proper :
+      Proper (eq ==> Eq_EvtSt ==> Eq_EvtSt ) ConsEvt.
+    Proof.
+      intros h1 h2 H_head t1 t2 H_tail.
+      subst; constructor; [reflexivity | assumption].
+    Qed.
+
+    Global Add Setoid EvtStream Eq_EvtSt Eq_EvtSt_equiv as EvtStreamSetoid.
+
+  Section DetTraces.
+    Parameter Det : det_rel steps_to_combined.
+    Lemma det_trace_prod : forall c m t1 t2, c ~~> (m, t1) -> c ~~> (m, t2) -> Eq_EvtSt t1 t2.
+      unfold "~~>", behavior; simpl.
+      cofix CH. 
+      intros.
+      pose proof Det (c, m) as Hdet.
+      unfold det_rel, steps_to_combined in Hdet.
+      inversion H; inversion H0; subst.
+      - destruct (Hdet (c', s') (c'0, s'0) a a0); try assumption.
+        + constructor.
+          * assumption.
+          * rewrite pair_equal_spec in H3; destruct H3; subst;
+            apply (CH c'0 s'0 st st0); assumption.
+      - apply produce_impl_canstep in H1.
+        contradiction.
+      - apply produce_impl_canstep in H5.
+        contradiction.
+      - apply Eq_EvtSt_refl.
+    Qed.
+  End DetTraces.
+End DetTheories.
